src/Triple.v
@@ -5,11 +5,13 @@ Unset Printing Implicit Defensive.
 From RDF Require Import Term.
 
 Section Triple.
-  Variable I B L: eqType.
+  Variable I B L: countType.
   Let term:= (term I B L).
   Let is_iri:= (@is_iri I B L).
   Let is_bnode:= (@is_bnode I B L).
   Let is_lit:= (@is_lit I B L).
+  Let code_term:= (@code_term I B L).
+  Let decode_term:= (@decode_term I B L).
 
   Record triple := mkTriple { subject : term
                             ; predicate : term
@@ -28,21 +30,55 @@ Section Triple.
          subst. by f_equal; apply eq_irrelevance.
   Qed.
 
-  Definition eqb_triple  (t1 t2 : triple) : bool :=
-    ((subject t1) == (subject t2)) &&
-      ((predicate t1) == (predicate t2)) &&
-      ((object t1) == (object t2)).
+  Definition code_triple (t : triple) :=
+    let (s,p,o,_,_,_) := t in
+    GenTree.Node 0 [:: (code_term s); (code_term p) ; (code_term o)].
 
-  Lemma triple_eqP : Equality.axiom eqb_triple.
-  Proof.
-    rewrite /Equality.axiom => x y.
-    apply: (iffP idP) => //= [| ->]; rewrite /eqb_triple; case: x y=> [s1 p1 o1 sin1 pin1 oin1] [s2 p2 o2 sin2 pin2 oin2] //=.
-    case/andP; case/andP=> /eqP eq_s/eqP eq_p/eqP eq_o.
-    apply: triple_inj; move=> //= {sin1 sin2 pin1 pin2 oin1 oin2}; by apply /eqP.
-    by rewrite !eq_refl //.
-  Qed.
+  (* Variable T : eqType. *)
+  (* Variable p : T -> bool. *)
+  (* Definition f ( x' : T) : option {x | p x}. *)
+  (* Proof. destruct (p x') eqn:E. *)
+  (*        - exact (Some (exist _ x' E)). *)
+  (*        - exact None. *)
+  (* Qed. *)
 
-  Canonical triple_eqType := EqType triple (EqMixin triple_eqP).
+  Definition decode_triple (x : GenTree.tree nat) : option triple.
+  Proof. destruct x eqn:E.
+         - exact None.
+         - destruct n as [| n'].
+           + destruct l as [| s [| p [| o]]] eqn:size.
+             * exact None.
+             * exact None.
+             * exact None.
+             * destruct l0.
+               -- destruct (decode_term s) as [dst | ] eqn:ds; destruct (decode_term p) as [dpt | ] eqn:dp ; destruct (decode_term o) as [ dot| ] eqn:do.
+                                                                                                                                                        destruct (is_in_ib dst) eqn:iib; destruct (is_in_i dpt) eqn:ii; destruct (is_in_ibl dot) eqn: ibl.
+                                                                                                                                                        ++ exact (Some (mkTriple iib ii ibl)).
+                                                                                                                                                        -- repeat exact None.
+                                                                                                                                                           all: exact None.
+  Defined.
+  
+  Lemma cancel_triple_encode : pcancel code_triple decode_triple.
+  Proof. case => s p o sib ii oibl. rewrite /code_triple /decode_triple.
+         (* rewrite *)
+         have cans: decode_term (code_term s) = Some s. apply cancel_code_decode.
+         have canp: decode_term (code_term p) = Some p. apply cancel_code_decode.
+         have cano: decode_term (code_term o) = Some o. apply cancel_code_decode.
+         rewrite /= !cans !canp !cano.
+         destruct s => //=; destruct p => //=; destruct o => //=.
+         all: f_equal; apply triple_inj; rewrite /=; reflexivity.
+         Qed. 
+         
+  Definition triple_eqMixin := PcanEqMixin cancel_triple_encode.
+  Definition triple_canChoiceMixin := PcanChoiceMixin cancel_triple_encode.
+  Definition triple_canCountMixin := PcanCountMixin cancel_triple_encode.
+
+  Canonical triple_eqType := Eval hnf in EqType triple triple_eqMixin.
+  Canonical triple_choiceType := Eval hnf in ChoiceType triple triple_canChoiceMixin.
+  Canonical triple_countType := Eval hnf in CountType triple triple_canCountMixin.
+
+  Definition triple_canPOrderMixin := PcanPOrderMixin (@pickleK triple_countType).
+  Canonical triple_POrderType := Eval hnf in POrderType tt triple triple_canPOrderMixin.
 
   Definition relabeling_triple (μ : B -> B) (t : triple) : triple :=
     let (s,p,o,sin,pin,oin) := t in
